coq/Frontend/LambdaNRA/LambdaAlg.v
@@ -1,3 +1,19 @@
+(*
+ * Copyright 2015-2016 IBM Corporation
+ *
+ * Licensed under the Apache License, Version 2.0 (the "License");
+ * you may not use this file except in compliance with the License.
+ * You may obtain a copy of the License at
+ *
+ * http://www.apache.org/licenses/LICENSE-2.0
+ *
+ * Unless required by applicable law or agreed to in writing, software
+ * distributed under the License is distributed on an "AS IS" BASIS,
+ * WITHOUT WARRANTIES OR CONDITIONS OF ANY KIND, either express or implied.
+ * See the License for the specific language governing permissions and
+ * limitations under the License.
+ *)
+
 Require Import String.
 Require Import List.
 Require Import Arith.
@@ -14,6 +30,7 @@ Section LambdaNRA.
   (* Lambda NRA *)
   Inductive lalg : Set :=
   | LAVar : string -> lalg (* Variable access *)
+  | LATable : string -> lalg
   | LAConst : data -> lalg
   | LABinop : binOp -> lalg -> lalg -> lalg
   | LAUnop : unaryOp -> lalg -> lalg
@@ -28,6 +45,7 @@ Section LambdaNRA.
   Tactic Notation "lalg_cases" tactic(first) ident(c) :=
   first;
   [ Case_aux c "LAVar"%string
+  | Case_aux c "LATable"%string
   | Case_aux c "LAConst"%string
   | Case_aux c "LABinop"%string
   | Case_aux c "LAUnop"%string
@@ -44,6 +62,7 @@ Section LambdaNRA.
   Definition  lalg_rect
               (P : lalg -> Type)
               (fvar : forall s : string, P (LAVar s))
+              (ftable : forall t : string, P (LATable t))
               (fconst : forall d : data, P (LAConst d))
               (fbinop : forall (b : binOp) (l : lalg), P l -> forall l0 : lalg, P l0 -> P (LABinop b l l0))
               (funop : forall (u : unaryOp) (l : lalg), P l -> P (LAUnop u l))
@@ -56,6 +75,7 @@ Section LambdaNRA.
       fix F (l : lalg) : P l :=
         match l as l0 return (P l0) with
         | LAVar s => fvar s
+        | LATable t => ftable t
         | LAConst d => fconst d
         | LABinop b l0 l1 => fbinop b l0 (F l0) l1 (F l1)
         | LAUnop u l0 => funop u l0 (F l0)
@@ -68,11 +88,15 @@ Section LambdaNRA.
   Definition lalg_ind (P : lalg -> Prop) := lalg_rect P.
   Definition lalg_rec (P:lalg->Set) := lalg_rect P.
 
+  (** Semantics of Lambda NRA *)
+
   Context (h:brand_relation_t).
+  Context (constant_env:list (string*data)).
 
   Fixpoint fun_of_lalg (env: bindings) (op:lalg) : option data :=
     match op with
     | LAVar x => edot env x
+    | LATable t => edot constant_env t
     | LAConst d => Some (normalize_data h d)
     | LABinop b op1 op2 => olift2 (fun d1 d2 => fun_of_binop h b d1 d2) (fun_of_lalg env op1) (fun_of_lalg env op2)
     | LAUnop u op1 =>
@@ -169,6 +193,7 @@ Section LambdaNRA.
   Lemma fun_of_lalg_normalized {op:lalg} {env:bindings} {o} :
     fun_of_lalg env op= Some o ->
     Forall (fun x => data_normalized h (snd x)) env ->
+    Forall (fun x => data_normalized h (snd x)) constant_env ->
     data_normalized h o.
   Proof.
     revert env o.
@@ -181,22 +206,29 @@ Section LambdaNRA.
       specialize (H0 _ H).
       simpl in H0.
       trivial.
+    - Case "LATable"%string.
+      unfold edot in H.
+      apply assoc_lookupr_in in H.
+      rewrite Forall_forall in H1.
+      specialize (H1 _ H).
+      simpl in H1.
+      trivial.
     - Case "LAConst"%string.
       invcs H.
       apply normalize_normalizes.
     - Case "LABinop"%string.
       unfold olift2 in H.
-      match_case_in H; intros; rewrite H1 in H; try discriminate.
       match_case_in H; intros; rewrite H2 in H; try discriminate.
+      match_case_in H; intros; rewrite H3 in H; try discriminate.
       eapply fun_of_binop_normalized; eauto.
     - Case "LAUnop"%string.
       unfold olift in H.
-      match_case_in H; intros; rewrite H1 in H; try discriminate.
+      match_case_in H; intros; rewrite H2 in H; try discriminate.
       eapply fun_of_unaryop_normalized; eauto.
     - Case "LAMap"%string.
       unfold olift in H.
-      match_case_in H; intros; rewrite H1 in H; try discriminate.
-      specialize (IHop2 _ _ H1 H0).
+      match_case_in H; intros; rewrite H2 in H; try discriminate.
+      specialize (IHop2 _ _ H2 H0 H1).
       unfold lift_oncoll in H.
       match_destr_in H.
       apply some_lift in H.
@@ -204,13 +236,13 @@ Section LambdaNRA.
       constructor.
       invcs IHop2.
       eapply (rmap_Forall e).
-      + apply H2.
+      + apply H3.
       + intros. eapply IHop1; eauto.
         apply Forall_app; auto.
     - Case "LAMapConcat"%string.
       unfold olift in H.
-      match_case_in H; intros; rewrite H1 in H; try discriminate.
-      specialize (IHop2 _ _ H1 H0).
+      match_case_in H; intros; rewrite H2 in H; try discriminate.
+      specialize (IHop2 _ _ H2 H0 H1).
       unfold lift_oncoll in H.
       match_destr_in H.
       apply some_lift in H.
@@ -219,36 +251,37 @@ Section LambdaNRA.
       invcs IHop2.
       unfold rmap_concat in e.
       eapply (oflat_map_Forall e).
-      + apply H2.
+      + apply H3.
       + intros.
         unfold oomap_concat in H.
-        match_case_in H; intros; rewrite H4 in H; try discriminate.
+        match_case_in H; intros; rewrite H5 in H; try discriminate.
         match_destr_in H.
         unfold omap_concat in H.
-        specialize (IHop1 _ _ H4).
+        specialize (IHop1 _ _ H5).
         cut_to IHop1.
         { invcs IHop1.
           eapply (rmap_Forall H).
-          - eapply H6.
+          - eapply H7.
           - intros.
             simpl in *.
-            unfold orecconcat in H5.
-            match_destr_in H5.
-            match_destr_in H5.
-            invcs H5.
+            unfold orecconcat in H6.
+            match_destr_in H6.
+            match_destr_in H6.
+            invcs H6.
             constructor.
             + apply Forall_sorted.
               apply Forall_app.
-              * invcs H3; trivial.
-              * invcs H7; trivial.
+              * invcs H4; trivial.
+              * invcs H8; trivial.
             + eauto.
         }
         apply Forall_app; trivial.
         constructor; trivial.
+        trivial.
     - Case "LAProduct"%string.
       unfold olift in H.
-      match_case_in H; intros; rewrite H1 in H; try discriminate.
-      specialize (IHop1 _ _ H1 H0).
+      match_case_in H; intros; rewrite H2 in H; try discriminate.
+      specialize (IHop1 _ _ H2 H0 H1).
       unfold lift_oncoll in H.
       match_destr_in H.
       apply some_lift in H.
@@ -257,35 +290,36 @@ Section LambdaNRA.
       invcs IHop1.
       unfold rmap_concat in e.
       eapply (oflat_map_Forall e).
-      + apply H2.
+      + apply H3.
       + intros.
         unfold oomap_concat in H.
-        match_case_in H; intros; rewrite H4 in H; try discriminate.
+        match_case_in H; intros; rewrite H5 in H; try discriminate.
         match_destr_in H.
         unfold omap_concat in H.
-        specialize (IHop2 _ _ H4).
+        specialize (IHop2 _ _ H5).
         cut_to IHop2.
         { invcs IHop2.
           eapply (rmap_Forall H).
-          - eapply H6.
+          - eapply H7.
           - intros.
             simpl in *.
-            unfold orecconcat in H5.
-            match_destr_in H5.
-            match_destr_in H5.
-            invcs H5.
+            unfold orecconcat in H6.
+            match_destr_in H6.
+            match_destr_in H6.
+            invcs H6.
             constructor.
             + apply Forall_sorted.
               apply Forall_app.
-              * invcs H3; trivial.
-              * invcs H7; trivial.
+              * invcs H4; trivial.
+              * invcs H8; trivial.
             + eauto.
         }
         trivial.
+        trivial.
     - Case "LASelect"%string.
       unfold olift in H.
-      match_case_in H; intros; rewrite H1 in H; try discriminate.
-      specialize (IHop2 _ _ H1 H0).
+      match_case_in H; intros; rewrite H2 in H; try discriminate.
+      specialize (IHop2 _ _ H2 H0 H1).
       unfold lift_oncoll in H.
       match_destr_in H.
       apply some_lift in H.
@@ -297,6 +331,52 @@ Section LambdaNRA.
       trivial.
   Qed.
   
+  Section LambdaNRAScope.
+
+    Fixpoint lalg_free_vars (e:lalg) :=
+      match e with
+      | LAConst d => nil
+      | LAVar v => v :: nil
+      | LATable t => nil
+      | LABinop bop e1 e2 => lalg_free_vars e1 ++ lalg_free_vars e2
+      | LAUnop uop e1 => lalg_free_vars e1
+      | LAMap (LALambda x e1) e2 =>
+        (remove string_eqdec x (lalg_free_vars e1)) ++ (lalg_free_vars e2)
+      | LAMapConcat (LALambda x e1) e2 =>
+        (remove string_eqdec x (lalg_free_vars e1)) ++ (lalg_free_vars e2)
+      | LAProduct e1 e2 =>
+        (lalg_free_vars e1) ++ (lalg_free_vars e2)
+      | LASelect (LALambda x e1) e2 =>
+        (remove string_eqdec x (lalg_free_vars e1)) ++ (lalg_free_vars e2)
+      end.
+
+  (* capture avoiding substitution *)
+    Fixpoint lalg_subst (e:lalg) (x:string) (e':lalg) : lalg :=
+      match e with
+      | LAConst d => LAConst d
+      | LAVar y => if y == x then e' else LAVar y
+      | LATable t => LATable t
+      | LABinop bop e1 e2 => LABinop bop
+                                   (lalg_subst e1 x e') 
+                                   (lalg_subst e2 x e')
+      | LAUnop uop e1 => LAUnop uop (lalg_subst e1 x e')
+      | LAMap (LALambda y e1) e2 =>
+        if (y == x)
+        then LAMap (LALambda y e1) (lalg_subst e2 x e')
+        else LAMap (LALambda y (lalg_subst e1 x e')) (lalg_subst e2 x e')
+      | LAMapConcat (LALambda y e1) e2 =>
+        if (y == x)
+        then LAMapConcat (LALambda y e1) (lalg_subst e2 x e')
+        else LAMapConcat (LALambda y (lalg_subst e1 x e')) (lalg_subst e2 x e')
+      | LAProduct e1 e2 =>
+        LAProduct (lalg_subst e1 x e') (lalg_subst e2 x e')
+      | LASelect (LALambda y e1) e2 =>
+        if (y == x)
+        then LASelect (LALambda y e1) (lalg_subst e2 x e')
+        else LASelect (LALambda y (lalg_subst e1 x e')) (lalg_subst e2 x e')
+      end.
+
+  End LambdaNRAScope.
 End LambdaNRA.
 
 Hint Rewrite @fun_of_lalg_lambda_lambda_eq : lalg.
@@ -308,6 +388,7 @@ Hint Rewrite @fun_of_lalg_select_eq : lalg.
 Tactic Notation "lalg_cases" tactic(first) ident(c) :=
   first;
   [ Case_aux c "LAVar"%string
+  | Case_aux c "LATable"%string
   | Case_aux c "LAConst"%string
   | Case_aux c "LABinop"%string
   | Case_aux c "LAUnop"%string
