coq/Frontend/LambdaNRA/LambdaAlgtoNRAEnv.v
@@ -1,3 +1,19 @@
+(*
+ * Copyright 2015-2016 IBM Corporation
+ *
+ * Licensed under the Apache License, Version 2.0 (the "License");
+ * you may not use this file except in compliance with the License.
+ * You may obtain a copy of the License at
+ *
+ * http://www.apache.org/licenses/LICENSE-2.0
+ *
+ * Unless required by applicable law or agreed to in writing, software
+ * distributed under the License is distributed on an "AS IS" BASIS,
+ * WITHOUT WARRANTIES OR CONDITIONS OF ANY KIND, either express or implied.
+ * See the License for the specific language governing permissions and
+ * limitations under the License.
+ *)
+
 Require Import String.
 Require Import List.
 Require Import Arith.
@@ -15,6 +31,7 @@ Section LambdaNRAtoNRAEnv.
   Fixpoint algenv_of_lalg (op:lalg) : algenv :=
     match op with
     | LAVar x => ANUnop (ADot x) ANEnv
+    | LATable x => ANGetConstant x
     | LAConst d => ANConst d
     | LABinop b op1 op2 => ANBinop b (algenv_of_lalg op1) (algenv_of_lalg op2)
     | LAUnop u op1 => ANUnop u (algenv_of_lalg op1)
@@ -30,9 +47,10 @@ Section LambdaNRAtoNRAEnv.
     end.
 
   Context (h:brand_relation_t).
+  Context (constant_env:list (string*data)).
     
   Theorem algenv_of_lalg_lambda_correct (env:bindings) (lop:lalg_lambda) (d:data) :
-    fun_of_lalg_lambda h env lop d = fun_of_algenv h nil (algenv_of_lalg_lambda lop) (drec env) d.
+    fun_of_lalg_lambda h constant_env env lop d = fun_of_algenv h constant_env (algenv_of_lalg_lambda lop) (drec env) d.
   Proof.
     destruct lop.
     revert env s d.
@@ -42,6 +60,9 @@ Section LambdaNRAtoNRAEnv.
     - Case "LAVar"%string.
       unfold edot, rec_concat_sort.
       rewrite assoc_lookupr_drec_sort.
+      trivial.
+    - Case "LATable"%string.
+      unfold edot, rec_concat_sort.
       trivial.
     - Case "LAConst"%string.
       trivial.
@@ -85,12 +106,12 @@ Section LambdaNRAtoNRAEnv.
       rewrite rec_sort_rec_sort_app1.
       trivial.
   Qed.
-      
+
   Definition eval_nraenv_q (Qe:algenv) (input:data) : option data :=
-    fun_of_algenv h nil Qe (drec nil) input.
+    fun_of_algenv h constant_env Qe (drec nil) input.
 
   Theorem eval_nraenv_q_correct (Q:lalg -> lalg) (input:data) :
-    eval_q h Q input = eval_nraenv_q (algenv_of_lalg_lambda (q_to_lambda Q)) input.
+    eval_q h constant_env Q input = eval_nraenv_q (algenv_of_lalg_lambda (q_to_lambda Q)) input.
   Proof.
     unfold eval_q, eval_nraenv_q.
     rewrite algenv_of_lalg_lambda_correct.
@@ -99,7 +120,7 @@ Section LambdaNRAtoNRAEnv.
 
 End LambdaNRAtoNRAEnv.
 
-  (* 
+(* 
 *** Local Variables: ***
 *** coq-load-path: (("../../../coq" "QCert")) ***
 *** End: ***
