coq/Tests/LambdaAlgTests.v
@@ -1,3 +1,19 @@
+(*
+ * Copyright 2015-2016 IBM Corporation
+ *
+ * Licensed under the Apache License, Version 2.0 (the "License");
+ * you may not use this file except in compliance with the License.
+ * You may obtain a copy of the License at
+ *
+ * http://www.apache.org/licenses/LICENSE-2.0
+ *
+ * Unless required by applicable law or agreed to in writing, software
+ * distributed under the License is distributed on an "AS IS" BASIS,
+ * WITHOUT WARRANTIES OR CONDITIONS OF ANY KIND, either express or implied.
+ * See the License for the specific language governing permissions and
+ * limitations under the License.
+ *)
+
 Require Import String.
 Require Import List.
 Require Import Arith.
@@ -52,12 +68,12 @@ Section LambdaNRATests.
     autorewrite with lalg.
     simpl.
     unfold olift.
-    destruct (fun_of_lalg h0 env P); trivial.
+    destruct (fun_of_lalg h0 cenv env P); trivial.
     unfold lift_oncoll.
     destruct d; trivial.
     induction l; simpl; trivial.
     autorewrite with lalg.
-    case_eq (@fun_of_lalg TrivialModel.trivial_foreign_runtime h0
+    case_eq (@fun_of_lalg TrivialModel.trivial_foreign_runtime h0 cenv
              (@app
                 (prod string
                    (@data (@foreign_runtime_data TrivialModel.trivial_foreign_runtime))) env
@@ -95,7 +111,7 @@ Section LambdaNRATests.
         simpl.
         destruct ((@rmap (@data TrivialModel.trivial_foreign_data)
                  (@data TrivialModel.trivial_foreign_data)
-                 (@fun_of_lalg_lambda TrivialModel.trivial_foreign_runtime h0 env
+                 (@fun_of_lalg_lambda TrivialModel.trivial_foreign_runtime h0 cenv env
                     (@LALambda TrivialModel.trivial_foreign_runtime
                        (String (Ascii.Ascii true false false false false true true false)
                           EmptyString)
